progress on funciton

refinedVST/typing/automation.v
@@ -173,6 +173,9 @@ Ltac liRStmt :=
       lazymatch s' with
       | Sassign _ _ => notypeclasses refine (tac_fast_apply (type_assign _ _ _ _ _) _)
       | Sset _ _ => notypeclasses refine (tac_fast_apply (type_set _ _ _ _ _ _) _)
+      | Ssequence _ _ => notypeclasses refine (tac_fast_apply (type_seq _ _ _ _ _) _)
+      | Sreturn $ Some _ => notypeclasses refine (tac_fast_apply (type_return_some _ _ _ _) _)
+      | Sreturn None => notypeclasses refine (tac_fast_apply (type_return_none _ _ _) _)
       | _ => fail "do_stmt: unknown stmt" s
       end
     end
@@ -407,56 +410,115 @@ Section automation_tests.
   liRStep.
   liRStep.
 Qed.
+End automation_tests.
 
 From VST.typing Require Import automation_test.
 
-Definition spec_f_ret_expr :=
-  fn(∀ () : (); <affine> True) → ∃ z : Z, int tint ; <absorb> ⌜z=42⌝.
-#[export] Instance CompSpecs : compspecs. make_compspecs prog. Defined.
-Definition Vprog : varspecs. mk_varspecs prog. Defined.
-Definition Delta := (func_tycontext f_f_ret_expr Vprog [] []).
+  Module f_test1.
+    Context `{!typeG Σ} {cs : compspecs} `{!externalGS OK_ty Σ}.
+  
+    Opaque local locald_denote.
 
-Goal forall Espec, ⊢ typed_function(A := ConstType _) Espec Delta f_f_ret_expr spec_f_ret_expr.
-Proof.
-  intros;
-  repeat iIntros "#?";
-  rewrite /typed_function.
-  iIntros ( x ). (* computes the ofe_car in x *) hnf in x. destruct x. simpl.
-  iSplit.
-  { iPureIntro; simpl. repeat constructor. }
-  let lsa := fresh "lsa" in
-  let lsb := fresh "lsb" in
-  let rho := fresh "rho" in
-  iIntros "!#" (lsa lsb rho). inv_vec lsb. inv_vec lsa.
+    Definition spec_f_ret_expr :=
+      fn(∀ () : (); <affine> True) → ∃ z : Z, int tint ; <absorb> ⌜z=42⌝.
+    Instance CompSpecs : compspecs. make_compspecs prog. Defined.
+    Definition Vprog : varspecs. mk_varspecs prog. Defined.
+    Definition Delta := (func_tycontext f_f_ret_expr Vprog [] []).
 
-  (* TODO go_higher here? *)
-  simpl.
+    Goal forall Espec, ⊢ typed_function(A := ConstType _) Espec Delta f_f_ret_expr spec_f_ret_expr.
+    Proof.
+      intros;
+      repeat iIntros "#?";
+      rewrite /typed_function.
+      iIntros ( x ). (* computes the ofe_car in x *) hnf in x. destruct x.
+      iSplit.
+      { iPureIntro; simpl. repeat constructor. }
+      let lsa := fresh "lsa" in
+      let lsb := fresh "lsb" in
+      let rho := fresh "rho" in
+      iIntros "!#" (lsa lsb rho). inv_vec lsb. inv_vec lsa.
+    
+      simpl. 
+      (* TODO go_higher here? *)
+      (* simpl. *)
 
-  rewrite -?(@monPred_at_emp environ_index mpred rho)
-          -?(@monPred_at_pure environ_index mpred rho) 
-          -?(monPred_at_affinely) 
-          -?monPred_at_sep 
-          -?monPred_wand_force.
+      rewrite -?(@monPred_at_emp environ_index mpred rho)
+              -?(@monPred_at_pure environ_index mpred rho) 
+              -?(monPred_at_affinely) 
+              -?monPred_at_sep 
+              -?monPred_wand_force.
 
-  Lemma go_higher : forall (P: assert) rho,
-    @bi_emp_valid (assert) P -> ⊢ monPred_at P rho.
-  Proof. 
-    intros ???.
-    destruct H as [H].
-    by iApply (H rho).
-  Qed.
+      Lemma go_higher : forall (P: assert) rho,
+        @bi_emp_valid (assert) P -> ⊢ monPred_at P rho.
+      Proof. 
+        intros ???.
+        destruct H as [H].
+        by iApply (H rho).
+      Qed.
 
-  iApply go_higher.
-  iStartProof.
+      iApply go_higher.
+      iStartProof.
 
-  liRStep.
-  liRStep.
-  liRStep.
-  liRStep.
-  liRStep.
-  liRStep.
-  liRStep.
-  repeat liRStep.
-  (* do Sreturn here *)
-  Admitted.
+      liRStep.
+      liRStep.
+      liRStep.
+      liRStep.
+      liRStep.
+      liRStep.
+      liRStep.
+      repeat liRStep.
+      (* do Sreturn here *)
+    Admitted.
+  End f_test1.
+
+  Module f_test2.
+    Context `{!typeG Σ} {cs : compspecs} `{!externalGS OK_ty Σ}.
+
+    Definition spec_f_temps :=
+      fn(∀ () : (); <affine> True) → ∃ z : Z, int tint ; <absorb> ⌜z=42⌝.
+    Local Instance CompSpecs : compspecs. make_compspecs prog. Defined.
+    Local Definition Vprog : varspecs. mk_varspecs prog. Defined.
+    Local Definition Delta := (func_tycontext f_f_temps Vprog [] []).
+
+    Goal forall Espec, ⊢ typed_function(A := ConstType _) Espec Delta f_f_temps spec_f_temps.
+    Proof.
+      intros;
+      repeat iIntros "#?";
+      rewrite /typed_function.
+      iIntros ( x ). (* computes the ofe_car in x *) hnf in x. destruct x.
+       (* simpl. *)
+      iSplit.
+      { iPureIntro; simpl. repeat constructor. }
+      let lsa := fresh "lsa" in
+      let lsb := fresh "lsb" in
+      let rho := fresh "rho" in
+      iIntros "!#" (lsa lsb rho). inv_vec lsb. inv_vec lsa.
+
+      simpl.
+      rewrite -?(@monPred_at_emp environ_index mpred rho)
+        -?(@monPred_at_pure environ_index mpred rho) 
+        -?(monPred_at_affinely) 
+        -?monPred_at_sep 
+        -?monPred_wand_force.
+
+    Lemma go_higher : forall (P: assert) rho,
+      @bi_emp_valid (assert) P -> ⊢ monPred_at P rho.
+    Proof. 
+      intros ???.
+      destruct H as [H].
+      by iApply (H rho).
+    Qed.
+
+    iApply go_higher.
+    iStartProof.
+
+
+
+      
+    repeat liRStep.
+    iIntros.
+    clear H.
+    repeat liRStep.
+    unfold IPM_JANNO.
+
 End automation_tests.
